Updated correctness predicates, module, and proofs

model/BTreesModule.v
@@ -9,7 +9,7 @@ Module Type CURSOR_TABLE.
  Parameter table: Type.
  Parameter cursor : Type.
  Parameter empty_t: table.
- Parameter empty_c: cursor.
+
  Parameter make_cursor: key -> table -> cursor.
  Parameter key_rel: key -> cursor -> bool.
  Parameter get: cursor -> option V.
@@ -17,14 +17,16 @@ Module Type CURSOR_TABLE.
  Parameter insert: cursor -> key -> V -> table.
  Parameter next: cursor -> cursor.
  Parameter prev: cursor -> cursor.
+ Parameter first_cursor: table -> cursor.
+ Parameter last_cursor: table -> cursor.
+
  Parameter abs_rel: table -> cursor -> Prop. (* Relationship between table and cursor *)
- Parameter cursor_valid: cursor -> Prop.
+
  Axiom make_cursor_rel: forall t k,
        abs_rel t (make_cursor k t).
- Axiom make_cursor_empty: forall k,
-       make_cursor k empty_t = empty_c.
- Axiom gempty:                 (* get-empty *)
-       get empty_c = None.
+
+ Axiom glast: forall t,                (* get-empty *)
+       get (last_cursor t) = None.
  Axiom gss: forall k v t,      (* get-set-same *)
        get (make_cursor k (set (make_cursor k t) v)) = Some v.
  Axiom gso: forall j k v t,    (* get-set-other *)
@@ -33,21 +35,23 @@ Module Type CURSOR_TABLE.
        get (make_cursor k (insert (make_cursor k t) k v)) = Some v.
  Axiom gio: forall j k v t,    (* get-insert-other *)
        j <> k -> get (make_cursor j (insert (make_cursor k t) k v)) = get (make_cursor j t).
- Axiom next_prev: forall c,
-       cursor_valid c -> prev (next c) = c.
+
+ Axiom next_prev: forall c t ,
+       abs_rel t c -> ~ (c = last_cursor t) -> prev (next c) = c.
 End CURSOR_TABLE.
 
-(* Currently missing some parts of the module specification because of cursor-key question *)
+(* NOT up to date *)
 Module BT_Table <: CURSOR_TABLE.
  Definition V := Type.
  Definition table := forest V.
  Definition cursor := BTrees.cursor V.
  Definition b : nat. Admitted.
  Definition key := Z.
- Definition empty : table := (BTrees.nil V).
+ Definition empty_t : table := (BTrees.nil V).
+ Definition empty_c : cursor := [].
  Definition get (k: key) (m: table) : option V := lookup V b k m.
  Definition set (k: key) (v: V) (m: table) : table := insert V b k v (make_cursor V b k m []).
- Theorem gempty: forall k, get k empty = None.
+ Theorem gempty: forall k, get k empty_t = None.
    Proof. intros. unfold get. unfold empty. Admitted.
  Theorem gss: forall k v t,  get k (set k v t) = Some v.
    Proof. Admitted.
